---
title: Bottling Computation Patterns
headerImg: sea.jpg
---

## Polymorphism and HOFs are the Secret Sauce 

**Refactor** arbitrary *repeated* code patterns ...

... into precisely *specified* and *reusable* **functions**

<br>
<br>
<br>
<br>
<br>
<br>
<br>
<br>
<br>
<br>

## EXERCISE: Iteration

Write a function that *squares* a list of `Int` 

```haskell
squares :: [Int] -> [Int]
squares ns = ???
```

When you are done you should see

```haskell
>>> squares [1,2,3,4,5]
[1,4,9,16,25]
```

<br>
<br>
<br>
<br>
<br>
<br>
<br>
<br>
<br>
<br>

## Pattern: Iteration

Next, lets write a function that converts a `String` to uppercase.

```haskell
>>> shout "hello"
"HELLO"
```

Recall that in Haskell, a `String` is just a `[Char]`.

```haskell
shout :: [Char] -> [Char]
shout = ???
```

[Hoogle][2] to see how to transform an individual `Char`

<br>
<br>
<br>
<br>
<br>
<br>
<br>
<br>
<br>
<br>

## Iteration

Common strategy: *iteratively* transform *each element* of input list 

Like humans and monkeys, `shout` and `squares` [share 93% of their DNA][3]

Super common *computation pattern*!

<br>
<br>
<br>
<br>
<br>
<br>
<br>
<br>
<br>
<br>

## Abstract Iteration "Pattern" into Function

Remember D.R.Y. (Don't repeat yourself)

**Step 1** Rename all variables to remove accidental *differences*

```haskell
-- rename 'squares' to 'foo'
foo []     = [] 
foo (x:xs) = (x * x)     : foo xs

-- rename 'shout' to 'foo'
foo []     = [] 
foo (x:xs) = (toUpper x) : foo xs
```

**Step 2** Identify what is *different*

- In `squares` we *transform* `x` to `x * x`

- In `shout` we *transform* `x` to `Data.Char.toUpper x`

**Step 3** Make *differences* a parameter

- Make *transform* a parameter `f` 

```haskell
foo f []     = [] 
foo f (x:xs) = (f x) : foo f xs
```

**Done** We have *bottled* the computation pattern as `foo` (aka `map`) 

```haskell
map f []     = [] 
map f (x:xs) = (f x) : map f xs
```

`map` bottles the common pattern of iteratively transforming a list:

![Fairy In a Bottle](/static/img/fairy.png)

<br>
<br>
<br>
<br>
<br>
<br>
<br>
<br>
<br>
<br>


## QUIZ 

What is the type of `map` ?

```haskell
map :: ???
map f []     = [] 
map f (x:xs) = (f x) : map f xs
```

**A.** `(Int -> Int) -> [Int] -> [Int]`

**B.** `(a -> a) -> [a] -> [a]`

**C.** `[a] -> [b]`

**D.** `(a -> b) -> [a] -> [b]`

**E.** `(a -> b) -> [a] -> [a]`

<br>
<br>
<br>
<br>
<br>
<br>
<br>
<br>
<br>
<br>

## The type precisely describes `map`

```haskell
>>> :type map
map :: (a -> b) -> [a] -> [b]
```

That is, `map` takes two inputs 

- a *transformer* of type `a -> b` 
- a *list* of values `[a]`

and it returns as output

- a list of values `[b]` 

that can only come by applying `f` to each element of the input list.

<br>
<br>
<br>
<br>
<br>
<br>
<br>
<br>

## Reusing the Pattern

Lets reuse the pattern by *instantiating* the transformer

### `shout` 

```haskell
-- OLD with recursion
shout :: [Char] -> [Char]
shout []     = []
shout (x:xs) = Char.toUpper x : shout xs

-- NEW with map
shout :: [Char] -> [Char]
shout xs = map (???) xs
``` 

### `squares` 

```haskell
-- OLD with recursion
squares :: [Int] -> [Int]
squares []     = []
squares (x:xs) = (x * x) : squares xs

-- NEW with map
squares :: [Int] -> [Int]
squares xs = map (???) xs 
``` 

<br>
<br>
<br>
<br>
<br>
<br>
<br>
<br>

## EXERCISE

Suppose I have the following type

```haskell
type Score = (Int, Int) -- pair of scores for Hw0, Hw1
```

Use `map` to write a function

```haskell
total :: [Score] -> [Int]
total xs = map (???) xs 
```

such that 

```haskell
>>> total [(10, 20), (15, 5), (21, 22), (14, 16)]
[30, 20, 43, 30]
```

<br>
<br>
<br>
<br>
<br>
<br>
<br>
<br>
<br>
<br>
<br>
<br>
<br>
<br>
<br>
<br>

## The Case of the Missing Parameter 

Note that we can write `shout` like this

```haskell
shout :: [Char] -> [Char]
shout = map Char.toUpper
```

Huh. No parameters? Can someone explain?

<br>
<br>
<br>
<br>
<br>
<br>
<br>
<br>
<br>
<br>
<br>

## The Case of the Missing Parameter 

In Haskell, the following all mean the same thing

Suppose we define a function

```haskell
add :: Int -> Int -> Int
add x y = x + y
```

Now the following all *mean the same thing*

```haskell
plus x y = add x y
plus x   = add x
plus     = add 
```

Why? *equational reasoning!* In general 

```haskell
foo x = e x

-- is equivalent to 

foo   = e
```

as long as `x` doesn't appear in `e`. 

Thus, to save some typing, we *omit* the extra parameter. 

<br>
<br>
<br>
<br>
<br>
<br>
<br>
<br>
<br>
<br>
<br>


## Pattern: Reduction

Computation patterns are *everywhere* lets revisit our old `sumList`

```haskell
sumList :: [Int] -> Int
sumList []     = 0
sumList (x:xs) = x + sumList xs
```

Next, a function that *concatenates* the `String`s in a list

```haskell
catList :: [String] -> String
catList []     = "" 
catList (x:xs) = x ++ (catList xs)
```

<br>
<br>
<br>
<br>
<br>
<br>
<br>
<br>
<br>
<br>
<br>

## Lets spot the pattern!

**Step 1** Rename

```haskell
foo []     = 0
foo (x:xs) = x + foo xs

foo []     = "" 
foo (x:xs) = x ++ foo xs
```

**Step 2** Identify what is *different*

1. ???

2. ???

**Step 3** Make *differences* a parameter

```haskell
foo p1 p2 []     = ???
foo p1 p2 (x:xs) = ???
```

<br>
<br>
<br>
<br>
<br>
<br>
<br>
<br>
<br>
<br>
<br>

## EXERCISE: Reduction/Folding

This pattern is commonly called *reducing* or *folding*

```haskell
foldr :: (a -> b -> b) -> b -> [a] -> b
foldr op base []     = base
foldr op base (x:xs) = op x (foldr op base xs)
```

Can you figure out how `sumList` and `catList` are just *instances* of `foldr`?

```haskell
sumList :: [Int] -> Int
sumList xs = foldr (?op) (?base) xs

catList :: [String] -> String 
catList xs = foldr (?op) (?base) xs
```

<br>
<br>
<br>
<br>
<br>
<br>
<br>
<br>
<br>
<br>
<br>


## Executing `foldr` 

To develop some intuition about `foldr` lets "run" it a few times by hand.

```haskell
foldr op b (a1:a2:a3:a4:[])
==> 
  a1 `op` (foldr op b (a2:a3:a4:[]))
==> 
  a1 `op` (a2 `op` (foldr op b (a3:a4:[])))
==> 
  a1 `op` (a2 `op` (a3 `op` (foldr op b (a4:[]))))
==> 
  a1 `op` (a2 `op` (a3 `op` (a4 `op` foldr op b [])))
==> 
  a1 `op` (a2 `op` (a3 `op` (a4 `op` b)))
```

Look how it *mirrors* the structure of lists!

- `(:)` is replaced by `op` 
- `[]` is replaced by `base`

So 

```haskell
foldr (+) 0 (x1:x2:x3:x4:[])
==> x1 + (x2 + (x3 + (x4 + 0))
``` 

<br>
<br>
<br>
<br>
<br>
<br>
<br>
<br>
<br>
<br>
<br>

## Typing `foldr` 

```haskell
foldr :: (a -> b -> b) -> b -> [a] -> b
foldr op base []     = base
foldr op base (x:xs) = op x (foldr op base xs)
```

`foldr` takes as input 

- a *reducer* function of type `a -> b -> b`
- a *base* value of type `b`
- a *list* of values to reduce `[a]`

and returns as output

- a *reduced* value `b`

<br>
<br>
<br>
<br>
<br>
<br>
<br>
<br>
<br>
<br>
<br>

## QUIZ

Recall the function to compute the `len` of a list

```haskell
len :: [a] -> Int
len []     = 0
len (x:xs) = 1 + len xs
```

Which of these is a valid implementation of `Len`

**A.** `len = foldr (\n -> n + 1) 0`

**B.** `len = foldr (\n m -> n + m) 0`

**C.** `len = foldr (\_ n -> n + 1) 0`

**D.** `len = foldr (\x xs -> 1 + len xs) 0`

**E.** All of the above

<br>
<br>
<br>
<br>
<br>
<br>
<br>
<br>
<br>
<br>
<br>

## The Missing Parameter Revisited

We wrote `foldr` as

```haskell
foldr :: (a -> b -> b) -> b -> [a] -> b
foldr op base []     = base
foldr op base (x:xs) = op x (foldr op base xs)
```

but can also write this

```haskell
foldr :: (a -> b -> b) -> b -> [a] -> b
foldr op base  = go 
  where
     go []     = base
     go (x:xs) = op x (go xs)
```

Can someone explain where the `xs` went *missing* ?

<br>
<br>
<br>
<br>
<br>
<br>
<br>
<br>
<br>
<br>
<br>

## Trees 

Recall the `Tree a` type from last time

```haskell
data Tree a 
  = Leaf 
  | Node a (Tree a) (Tree a)
```

For example here's a tree

```haskell
tree2 :: Tree Int
tree2 = Node 2 Leaf Leaf

tree3 :: Tree Int
tree3 = Node 3 Leaf Leaf

tree123 :: Tree Int
tree123 = Node 1 tree2 tree3 
```

<br>
<br>
<br>
<br>
<br>
<br>
<br>
<br>
<br>
<br>
<br>

## Some Functions on Trees

Lets write a function to compute the `height` of a tree

```haskell
height :: Tree a -> Int
height Leaf         = 0
height (Node x l r) = 1 + max (height l) (height l)
```

Here's another to *sum* the leaves of a tree:

```haskell
sumTree :: Tree Int -> Int
sumTree Leaf         = ???
sumTree (Node x l r) = ???
```

Gathers all the elements that occur as leaves of the tree:

```haskell
toList :: Tree a -> [a] 
toList Leaf         = ??? 
toList (Node x l r) = ???
```

Lets give it a whirl

```haskell
>>> height tree123
2 

>>> sumTree tree123
6

>>> toList tree123
[1,2,3]
```

<br>
<br>
<br>
<br>
<br>
<br>
<br>
<br>
<br>
<br>
<br>

## Pattern: Tree Fold 

Can you spot the pattern? Those three functions are almost the same!

**Step 1:** Rename to maximize similarity

```haskell
-- height
foo Leaf         = 0
foo (Node x l r) = 1 + max (foo l) (foo l)

-- sumTree
foo Leaf         = 0
foo (Node x l r) = foo l + foo r

-- toList
foo Leaf         = []
foo (Node x l r) = x : foo l ++ foo r
```

**Step 2:** Identify the differences

1. ???
2. ???

 
**Step 3** Make *differences* a parameter

```haskell
foo p1 p2 Leaf         = ???
foo p1 p2 (Node x l r) = ???
```

<br>
<br>
<br>
<br>
<br>
<br>
<br>
<br>
<br>
<br>
<br>

## Pattern: Folding on Trees

```haskell
tFold op b Leaf         = b 
tFold op b (Node x l r) = op x (tFold op b l) (tFold op b r)
```

Lets try to work out the type of `tFold`!

```haskell
tFold :: t_op -> t_b -> Tree a -> t_out
```

<br>
<br>
<br>
<br>
<br>
<br>
<br>
<br>
<br>


## QUIZ 

Suppose that `t :: Tree Int`. 

What does `tFold (\x y z -> y + z) 1 t` return?

**a.** `0`

**b.** the *largest*  element in the tree `t`

**c.** the *height*   of the tree `t`

**d.** the *number-of-leaves* of the tree `t`

**e.** type *error*

<br>
<br>
<br>
<br>
<br>
<br>
<br>
<br>
<br>

## EXERCISE 

Write a function to compute the _largest_ element in a tree 
or `0` if tree is empty or all negative.

```haskell
treeMax :: Tree Int -> Int
treeMax t = tFold f b t 
  where 
     f    = ??? 
     b    = ???
```

<br>
<br>
<br>
<br>
<br>
<br>
<br>
<br>
<br>

## Map over Trees

We can also write a `tmap` equivalent of `map` for `Tree`s 

```haskell
treeMap :: (a -> b) -> Tree a -> Tree b
treeMap f (Leaf x)   = Leaf (f x)
treeMap f (Node l r) = Node (treeMap f l) (treeMap f r)
```

which gives

```haskell
>>> treeMap (\n -> n * n) tree123     -- square all elements of tree
Node 1 (Node 4 Leaf Leaf) (Node 9 Leaf Leaf)
```

<br>
<br>
<br>
<br>
<br>
<br>
<br>
<br>
<br>

## EXERCISE 

Recursion is **HARD TO READ** do we really have to use it ?

Lets rewrite `treeMap` using `tFold` !

```haskell
treeMap :: (a -> b) -> Tree a -> Tree b
treeMap f t = tFold op base t 
  where 
     op     = ??? 
     base   = ??? 
```

When you are done, we should get

```haskell
>>> animals = Node "cow" (Node "piglet" Leaf Leaf) (Leaf "hippo" Leaf Leaf)
>>> treeMap reverse animals
Node "woc" (Node "telgip" Leaf Leaf) (Leaf "oppih" Leaf Leaf)
```

<br>
<br>
<br>
<br>
<br>
<br>
<br>
<br>
<br>

## Examples: `foldDir`

```haskell
data Dir a 
  = Fil a             -- ^ A single file named `a`
  | Sub a [Dir a]     -- ^ A sub-directory name `a` with contents `[Dir a]`

data DirElem a 
  = SubDir a          -- ^ A single Sub-Directory named `a`
  | File a            -- ^ A single File named `a` 

foldDir :: ([a] -> r -> DirElem a -> r) -> r -> Dir a -> r
foldDir f r0 dir = go [] r0 dir  
  where
      go stk r (Fil a)    = f stk r (File a)  
      go stk r (Sub a ds) = L.foldl' (go stk') r' ds                          
        where 
            r'   = f stk r (SubDir a)  
            stk' = a:stk
```

`foldDir` takes as input 

- an *accumulator* `f` of type `[a] -> r -> DirElem a -> r` 

  - takes as *input* the path `[a]` , the current result `r`, the next `DirElem [a]` 

  - and returns as *output* the new result `r`

- an *initial* value of the result `r0` and 

- directory to fold over `dir`

And returns the result of running the *accumulator* over the whole `dir`.

<br>
<br>
<br>
<br>
<br>
<br>
<br>
<br>
<br>

## Examples: Spotting Patterns In The "Real" World

**These patterns in "toy" functions appear regularly in "real" code**

1. Start with beginner's version riddled with [explicit recursion](swizzle-v0.html).

2. Spot the patterns and eliminate recursion using [HOFs](swizzle-v1.html).

3. Finally refactor the code to "swizzle" and "unswizzle" [without duplication](swizzle-v2.html).

**Try it yourself**

* Rewrite the code that swizzles `Char` to use the `Map k v` type in `Data.Map`

<br>
<br>
<br>
<br>
<br>
<br>
<br>
<br>
<br>

## Which is more readable? HOFs or Recursion

At first, *recursive* versions of `shout` and `squares` are easier to follow

- `fold` takes a bit of getting used to!

With practice, the *higher-order* versions become easier

- only have to understand specific operations

- recursion is lower-level & have to see "loop" structure 

- worse, potential for making silly off-by-one errors 

Indeed, HOFs were the basis of `map/reduce` and the [big-data revolution][4]

- Can *parallelize* and *distribute* computation patterns [just once][5]

- [Reuse][4] across hundreds or thousands of instances!

[1]: http://hackage.haskell.org/packages/archive/base/latest/doc/html/Data-List.html "Data.List"
[2]: http://haskell.org/hoogle "Hoogle Query: Char -> Char"
[3]: http://www.livescience.com/health/070412_rhesus_monkeys.html
[4]: http://en.wikipedia.org/wiki/MapReduce "MapReduce"
[5]: https://www.usenix.org/event/osdi04/tech/full_papers/dean/dean.pdf